src/Std/Data/DHashMap/Internal/MyRawLemmas.lean
@@ -35,6 +35,19 @@ theorem isEmpty_modify [LawfulBEq α] (h : m.1.WF) {k : α} {f : β k → β k} 
     (m.modify k f).1.isEmpty = m.1.isEmpty := by
   simp_to_model using List.isEmpty_modifyKey
 
+section Alter
+
+-- theorem constAlter_eq_alter [LawfulBEq α] {β : Type v} (m : Raw₀ α (fun _ => β)) (a : α)
+--     (f : Option β → Option β) : Const.alter m a f = m.alter a f := by
+--   simp_to_model using List.constAlterKey_eq_alterKey
+
+-- theorem alter_empty [LawfulBEq α] {k : α} {f : Option (β k) → Option (β k)} :
+--     empty.alter k f =
+--     match f none with
+--     | none => empty
+--     | some v => empty.insert k v := by
+--   simp_to_model using List.alterKey_nil
+
 @[simp]
 theorem isEmpty_alter [LawfulBEq α] (h : m.1.WF) {k : α} {f : Option (β k) → Option (β k)} :
     (m.alter k f).1.isEmpty = ((m.erase k).1.isEmpty && (f (m.get? k)).isNone) := by
@@ -43,6 +56,48 @@ theorem isEmpty_alter [LawfulBEq α] (h : m.1.WF) {k : α} {f : Option (β k) �
 theorem contains_alter [LawfulBEq α] (h : m.1.WF) {k k' : α} {f : Option (β k) → Option (β k)} :
     (m.alter k f).contains k' = if k == k' then (f (m.get? k)).isSome else m.contains k' := by
   simp_to_model using List.containsKey_alterKey
+
+theorem size_alter [LawfulBEq α] (h : m.1.WF) {k : α} {f : Option (β k) → Option (β k)} :
+    (m.alter k f).1.size =
+    if m.contains k && (f (m.get? k)).isNone then
+      m.1.size - 1
+    else if !m.contains k && (f (m.get? k)).isSome then
+      m.1.size + 1
+    else
+      m.1.size := by
+  simp_to_model using List.length_alterKey'
+
+theorem size_alter_eq_add_one [LawfulBEq α] (h : m.1.WF) {k : α} {f : Option (β k) → Option (β k)}
+    (h₁ : m.contains k = false) (h₂: (f (m.get? k)).isSome) :
+    (m.alter k f).1.size = m.1.size + 1 := by
+  simp [size_alter, h, h₁, h₂]
+
+theorem size_alter_eq_sub_one [LawfulBEq α] (h : m.1.WF) {k : α} {f : Option (β k) → Option (β k)}
+    (h₁ : m.contains k) (h₂: (f (m.get? k)).isNone) :
+    (m.alter k f).1.size = m.1.size - 1 := by
+  simp [size_alter, h, h₁, h₂]
+
+theorem size_alter_eq_self [LawfulBEq α] (h : m.1.WF) {k : α} {f : Option (β k) → Option (β k)}
+    (h₁ : m.contains k = false) (h₂: (f (m.get? k)).isNone) :
+    (m.alter k f).1.size = m.1.size := by
+  simp [size_alter, h, h₁, h₂]
+
+theorem size_alter_eq_self' [LawfulBEq α] (h : m.1.WF) {k : α} {f : Option (β k) → Option (β k)}
+    (h₁ : m.contains k) (h₂: (f (m.get? k)).isSome) :
+    (m.alter k f).1.size = m.1.size := by
+  simp [size_alter, h, h₁, Option.isSome_iff_ne_none.mp h₂]
+
+theorem size_alter_le_size [LawfulBEq α] (h : m.1.WF) {k : α} {f : Option (β k) → Option (β k)} :
+    (m.alter k f).1.size ≤ m.1.size + 1 := by
+  simp [size_alter, h]
+  split <;> try split
+  all_goals omega
+
+theorem size_le_size_alter [LawfulBEq α] (h : m.1.WF) {k : α} {f : Option (β k) → Option (β k)} :
+    m.1.size - 1 ≤ (m.alter k f).1.size := by
+  simp [size_alter, h]
+  split <;> try split
+  all_goals omega
 
 theorem get?_alter [LawfulBEq α] (h : m.1.WF) {k k' : α} {f : Option (β k) → Option (β k)} :
     (m.alter k f).get? k' = if h : k == k' then
@@ -60,26 +115,13 @@ theorem get_alter [LawfulBEq α] (h : m.1.WF) {k k' : α} {f : Option (β k) →
     else
       haveI h' : m.contains k' := by rwa [contains_alter _ h, if_neg heq] at hc
       m.get k' h' := by
-  have := get?_alter m (k' := k') (f := f) h
-  rw [get?_eq_some_get _ h.alter₀ (h' := hc)] at this
-  · split
-    · next heq =>
-      cases eq_of_beq heq
-      apply Option.some_inj.mp
-      simp_all
-    · next heq =>
-      apply Option.some_inj.mp
-      simp_all only [Bool.false_eq_true, Function.comp_apply, dite_false]
-      rw [get?_eq_some_get m h]
+  simp_to_model using List.getValueCast_alterKey
 
 theorem get_alter_self [LawfulBEq α] (h : m.1.WF) {k : α} {f : Option (β k) → Option (β k)}
     {hc : (m.alter k f).contains k} :
     haveI h' : (f (m.get? k)).isSome := by rwa [contains_alter _ h, beq_self_eq_true] at hc
     (m.alter k f).get k hc = (f (m.get? k)).get h' := by
-  rw [get_alter _ h]
-  simp only [beq_self_eq_true, reduceDIte, cast_eq]
-
-theorem cast_eq_id {α : Type u} : cast (rfl : α = α) = id := by rfl
+  simp_to_model using List.getValueCast_alterKey_self
 
 theorem get!_alter [LawfulBEq α] {k k' : α} (h : m.1.WF) [Inhabited (β k')] {f : Option (β k) → Option (β k)} :
     (m.alter k f).get! k' =
@@ -88,12 +130,7 @@ theorem get!_alter [LawfulBEq α] {k k' : α} (h : m.1.WF) [Inhabited (β k')] {
       cast (congrArg β (eq_of_beq heq)) <| (f (m.get? k)).get!
     else
       m.get! k' := by
-  simp only [get!_eq_get!_get?, h.alter₀, h, get?_alter, beq_iff_eq, Function.comp_apply]
-  split
-  · next heq =>
-    cases eq_of_beq heq
-    simp only [cast_eq]
-  · rfl
+  simp_to_model using List.getValueCast!_alterKey
 
 theorem getD_alter [LawfulBEq α] {k k' : α} {v : β k'} (h : m.1.WF) {f : Option (β k) → Option (β k)} :
     (m.alter k f).getD k' v =
@@ -101,12 +138,7 @@ theorem getD_alter [LawfulBEq α] {k k' : α} {v : β k'} (h : m.1.WF) {f : Opti
       f (m.get? k) |>.map (cast (congrArg β <| eq_of_beq heq)) |>.getD v
     else
       m.getD k' v := by
-  simp only [getD_eq_getD_get?, h.alter₀, h, get?_alter, beq_iff_eq, Function.comp_apply]
-  split
-  · next heq =>
-    cases eq_of_beq heq
-    simp only [cast_eq_id, Option.map_id]
-  · rfl
+  simp_to_model using List.getValueCastD_alterKey
 
 theorem getD_alter_self [LawfulBEq α] {k : α} {v : β k} (h : m.1.WF) {f : Option (β k) → Option (β k)} :
     (m.alter k f).getD k v = (f (m.get? k)).getD v := by
@@ -126,13 +158,7 @@ theorem getKey!_alter [LawfulBEq α] [Inhabited α] {k k' : α} (h : m.1.WF) {f 
       if (f (m.get? k)).isSome then k else panic ""
     else
       m.getKey! k' := by
-  simp [getKey!_eq_get!_getKey?, getKey?_alter, h, h.alter₀]
-  split
-  · next heq =>
-    cases eq_of_beq heq
-    split <;> rfl
-  · next heq =>
-    rfl
+  simp_to_model using List.getKey!_alterKey
 
 theorem getKey_alter [LawfulBEq α] [Inhabited α] {k k' : α} (h : m.1.WF) {f : Option (β k) → Option (β k)}
     (hc : (m.alter k f).contains k') :
@@ -169,16 +195,416 @@ theorem getKeyD_alter [LawfulBEq α] {k k' d : α} (h : m.1.WF) {f : Option (β 
 
 namespace Const
 
-variable {β : Type v} [EquivBEq α] [LawfulHashable α]
+variable {β : Type v} [EquivBEq α] [LawfulHashable α] (m : Raw₀ α (fun _ => β))
+
+-- theorem alter_empty {k : α} {f : Option β → Option β} :
+--     Const.alter empty k f =
+--     match f none with
+--     | none => empty
+--     | some v => empty.insert k v := by
+--   simp_to_model using List.Const.alterKey_nil
+
+@[simp]
+theorem isEmpty_alter (h : m.1.WF)  {k : α} {f : Option β → Option β} :
+    (Const.alter m k f).1.isEmpty ↔ (m.erase k).1.isEmpty ∧ f (Const.get? m k) = none := by
+  simp_to_model using List.Const.isEmpty_alterKey
+
+theorem contains_alter (h : m.1.WF) {k k' : α} {f : Option β → Option β} :
+    (Const.alter m k f).contains k' = if k == k' then (f (Const.get? m k)).isSome else m.contains k' := by
+  simp_to_model using List.Const.containsKey_alterKey
+
+theorem size_alter (h : m.1.WF) {k : α} {f : Option β → Option β} :
+    (Const.alter m k f).1.size =
+    if m.contains k && (f (Const.get? m k)).isNone then
+      m.1.size - 1
+    else if !m.contains k && (f (Const.get? m k)).isSome then
+      m.1.size + 1
+    else
+      m.1.size := by
+  simp_to_model using List.Const.length_alterKey'
+
+theorem size_alter_eq_add_one (h : m.1.WF) {k : α} {f : Option β → Option β}
+    (h₁ : m.contains k = false) (h₂: (f (Const.get? m k)).isSome) :
+    (Const.alter m k f).1.size = m.1.size + 1 := by
+  simp [size_alter, h, h₁, h₂]
+
+theorem size_alter_eq_sub_one (h : m.1.WF) {k : α} {f : Option β → Option β}
+    (h₁ : m.contains k) (h₂: (f (Const.get? m k)).isNone) :
+    (Const.alter m k f).1.size = m.1.size - 1 := by
+  simp [size_alter, h, h₁, h₂]
+
+theorem size_alter_eq_self (h : m.1.WF) {k : α} {f : Option β → Option β}
+    (h₁ : m.contains k = false) (h₂: (f (Const.get? m k)).isNone) :
+    (Const.alter m k f).1.size = m.1.size := by
+  simp [size_alter, h, h₁, h₂]
+
+theorem size_alter_eq_self' (h : m.1.WF) {k : α} {f : Option β → Option β}
+    (h₁ : m.contains k) (h₂: (f (Const.get? m k)).isSome) :
+    (Const.alter m k f).1.size = m.1.size := by
+  simp [size_alter, h, h₁, Option.isSome_iff_ne_none.mp h₂]
+
+theorem size_alter_le_size [LawfulBEq α] (h : m.1.WF) {k : α} {f : Option β → Option β} :
+    (Const.alter m k f).1.size ≤ m.1.size + 1 := by
+  simp [size_alter, h]
+  split <;> try split
+  all_goals omega
+
+theorem size_le_size_alter [LawfulBEq α] (h : m.1.WF) {k : α} {f : Option β → Option β} :
+    m.1.size - 1 ≤ (Const.alter m k f).1.size := by
+  simp [size_alter, h]
+  split <;> try split
+  all_goals omega
+
+theorem get?_alter (h : m.1.WF) {k k' : α} {f : Option β → Option β} :
+    Const.get? (Const.alter m k f) k' = if k == k' then
+      f (Const.get? m k)
+    else
+      Const.get? m k' := by
+  simp_to_model using List.Const.getValue?_alterKey
+
+theorem get_alter (h : m.1.WF) {k k' : α} {f : Option β → Option β}
+    (hc : (Const.alter m k f).contains k') :
+    Const.get (Const.alter m k f) k' hc =
+    if heq : k == k' then
+      haveI h' : (f (Const.get? m k)).isSome := by rwa [contains_alter _ h, if_pos heq] at hc
+      (f (Const.get? m k)).get <| h'
+    else
+      haveI h' : m.contains k' := by rwa [contains_alter _ h, if_neg heq] at hc
+      Const.get m k' h' := by
+  simp_to_model using List.Const.getValue_alterKey
+
+theorem get_alter_self (h : m.1.WF) {k : α} {f : Option β → Option β}
+    {hc : (Const.alter m k f).contains k} :
+    haveI h' : (f (Const.get? m k)).isSome := by rwa [contains_alter _ h, BEq.refl] at hc
+    Const.get (Const.alter m k f) k hc = (f (Const.get? m k)).get h' := by
+  simp_to_model using List.Const.getValue_alterKey_self
+
+theorem cast_eq_id {α : Type u} : cast (rfl : α = α) = id := by rfl
+
+theorem get!_alter {k k' : α} (h : m.1.WF) [Inhabited β] {f : Option β → Option β} :
+    Const.get! (Const.alter m k f) k' =
+    if k == k' then
+      (f (Const.get? m k)).get!
+    else
+      Const.get! m k' := by
+  simp_to_model using List.Const.getValue!_alterKey
+
+theorem getD_alter {k k' : α} {v : β} (h : m.1.WF) {f : Option β → Option β} :
+    Const.getD (Const.alter m k f) k' v =
+    if k == k' then
+      f (Const.get? m k) |>.getD v
+    else
+      Const.getD m k' v := by
+  simp_to_model using List.Const.getValueD_alterKey
+
+theorem getD_alter_self {k : α} {v : β} (h : m.1.WF) {f : Option β → Option β} :
+    Const.getD (Const.alter m k f) k v = (f (Const.get? m k)).getD v := by
+  simp only [h, getD_alter, BEq.refl, reduceIte]
+
+theorem getKey?_alter (h : m.1.WF) {k k' : α} {f : Option β → Option β} :
+    (Const.alter m k f).getKey? k' =
+    if k == k' then
+      if (f (Const.get? m k)).isSome then some k else none
+    else
+      m.getKey? k' := by
+  simp_to_model using List.Const.getKey?_alterKey
+
+theorem getKey!_alter [Inhabited α] {k k' : α} (h : m.1.WF) {f : Option β → Option β} :
+    (Const.alter m k f).getKey! k' =
+    if k == k' then
+      if (f (Const.get? m k)).isSome then k else panic ""
+    else
+      m.getKey! k' := by
+  simp_to_model using List.Const.getKey!_alterKey
+
+theorem getKey_alter [Inhabited α] {k k' : α} (h : m.1.WF) {f : Option β → Option β}
+    (hc : (Const.alter m k f).contains k') :
+    (Const.alter m k f).getKey k' hc =
+    if heq : k == k' then
+      k
+    else
+      haveI h' : m.contains k' := by rwa [contains_alter _ h, if_neg heq] at hc
+      m.getKey k' h' := by
+  simp_to_model using List.Const.getKey_alterKey
+
+theorem getKeyD_alter {k k' d : α} (h : m.1.WF) {f : Option β → Option β} :
+    (Const.alter m k f).getKeyD k' d =
+    if k == k' then
+      if (f (Const.get? m k)).isSome then k else d
+    else
+      m.getKeyD k' d := by
+  simp_to_model using List.Const.getKeyD_alterKey
+
+end Const
+
+end Alter
+
+section Modify
+
+variable [LawfulBEq α]
+
+-- theorem constModify_eq_modify {β : Type v} (m : Raw₀ α (fun _ => β)) (a : α)
+--     (f : β → β) : Const.modify m a f = m.modify a f := by
+--   simp_to_model using List.constModifyKey_eq_modifyKey
+
+-- @[simp]
+-- theorem modify_empty [LawfulBEq α] {k : α} {f : β k → β k} : empty.modify k f = empty := by
+--   simp_to_model using List.modifyKey_nil
+
+-- theorem modify_of_not_mem [LawfulBEq α] {k : α} {f g : β k → β k} (h : m.contains k = false) :
+--     m.modify k f = m := by
+--   simp_to_model using List.modifyKey_of_not_mem
+
+theorem contains_modify (h : m.1.WF) {k k' : α} {f : β k → β k} :
+    (m.modify k f).contains k' = m.contains k' := by
+  simp_to_model using List.containsKey_modifyKey
+
+theorem size_modify (h : m.1.WF) {k : α} {f : β k → β k} :
+    (m.modify k f).1.size = m.1.size := by
+  simp_to_model using List.length_modifyKey
+
+theorem get?_modify (h : m.1.WF) {k k' : α} {f : β k → β k} :
+    (m.modify k f).get? k' = if h : k == k' then
+      (cast (congrArg (Option ∘ β) (eq_of_beq h)) ((m.get? k).map f))
+    else
+      m.get? k' := by
+  simp_to_model using List.getValueCast?_modifyKey
+
+@[simp]
+theorem get?_modify_self (h : m.1.WF) {k : α} {f : β k → β k} :
+    (m.modify k f).get? k = (m.get? k).map f := by
+  simp_to_model using List.getValueCast?_modifyKey_self
+
+theorem get_modify (h : m.1.WF) {k k' : α} {f : β k → β k}
+    (hc : (m.modify k f).contains k') :
+    (m.modify k f).get k' hc =
+    if heq : k == k' then
+      haveI h' : m.contains k := by rwa [contains_modify _ h, ← eq_of_beq heq] at hc
+      cast (congrArg β (eq_of_beq heq)) <| f (m.get k h')
+    else
+      haveI h' : m.contains k' := by rwa [contains_modify _ h] at hc
+      m.get k' h' := by
+  simp_to_model using List.getValueCast_modifyKey
+
+@[simp]
+theorem get_modify_self (h : m.1.WF) {k : α} {f : β k → β k} {hc : (m.modify k f).contains k} :
+    haveI h' : m.contains k := by rwa [contains_modify _ h] at hc
+    (m.modify k f).get k hc = f (m.get k h') := by
+  simp_to_model using List.getValueCast_modifyKey_self
+
+theorem get!_modify (h : m.1.WF) {k k' : α} [hi : Inhabited (β k')] {f : β k → β k} :
+    (m.modify k f).get! k' =
+    if heq : k == k' then
+      haveI : Inhabited (β k) := ⟨cast (congrArg β <| eq_of_beq heq).symm default⟩
+      -- not correct if f does not preserve default: ... f (m.get! k)
+      -- possible alternative: write ... (m.getD k (cast ⋯ default))
+      m.get? k |>.map f |>.map (cast (congrArg β (eq_of_beq heq))) |>.get!
+    else
+      m.get! k' := by
+  simp_to_model using List.getValueCast!_modifyKey
+
+@[simp]
+theorem get!_modify_self (h : m.1.WF) {k : α} [Inhabited (β k)] {f : β k → β k} :
+    (m.modify k f).get! k = ((m.get? k).map f).get! := by
+  simp_to_model using List.getValueCast!_modifyKey_self
+
+theorem getD_modify (h : m.1.WF) {k k' : α} {v : β k'} {f : β k → β k} :
+    (m.modify k f).getD k' v =
+    if heq : k == k' then
+      m.get? k |>.map f |>.map (cast (congrArg β <| eq_of_beq heq)) |>.getD v
+    else
+      m.getD k' v := by
+  simp_to_model using List.getValueCastD_modifyKey
+
+@[simp]
+theorem getD_modify_self (h : m.1.WF) {k : α} {v : β k} {f : β k → β k} :
+    (m.modify k f).getD k v = ((m.get? k).map f).getD v := by
+  simp_to_model using List.getValueCastD_modifyKey_self
+
+theorem getKey?_modify (h : m.1.WF) {k k' : α} {f : β k → β k} :
+    (m.modify k f).getKey? k' =
+    if k == k' then
+      if m.contains k then some k else none
+    else
+      m.getKey? k' := by
+  simp_to_model using List.getKey?_modifyKey
+
+theorem getKey?_modify_self (h : m.1.WF) {k : α} {f : β k → β k} :
+    (m.modify k f).getKey? k = if m.contains k then some k else none := by
+  simp_to_model using List.getKey?_modifyKey_self
+
+theorem getKey!_modify (h : m.1.WF) [Inhabited α] {k k' : α} {f : β k → β k} :
+    (m.modify k f).getKey! k' =
+    if k == k' then
+      if m.contains k then k else panic ""
+    else
+      m.getKey! k' := by
+  simp_to_model using List.getKey!_modifyKey
+
+theorem getKey!_modify_self (h : m.1.WF) [Inhabited α] {k : α} {f : β k → β k} :
+    (m.modify k f).getKey! k = if m.contains k then k else panic "" := by
+  simp_to_model using List.getKey!_modifyKey_self
+
+theorem getKey_modify (h : m.1.WF) [Inhabited α] {k k' : α} {f : β k → β k}
+    (hc : (m.modify k f).contains k') :
+    (m.modify k f).getKey k' hc =
+    if heq : k == k' then
+      k
+    else
+      haveI h' : m.contains k' := by rwa [contains_modify _ h] at hc
+      m.getKey k' h' := by
+  simp_to_model using List.getKey_modifyKey
+
+@[simp]
+theorem getKey_modify_self (h : m.1.WF) [Inhabited α] {k : α} {f : β k → β k}
+    (hc : (m.modify k f).contains k) : (m.modify k f).getKey k hc = k := by
+  simp_to_model using List.getKey_modifyKey_self
+
+theorem getKeyD_modify (h : m.1.WF) {k k' d : α} {f : β k → β k} :
+    (m.modify k f).getKeyD k' d =
+    if k == k' then
+      if m.contains k then k else d
+    else
+      m.getKeyD k' d := by
+  simp_to_model using List.getKeyD_modifyKey
+
+theorem getKeyD_modify_self (h : m.1.WF) [Inhabited α] {k d : α} {f : β k → β k} :
+    (m.modify k f).getKeyD k d = if m.contains k then k else d := by
+  simp_to_model using List.getKeyD_modifyKey_self
+
+namespace Const
+
+variable {β : Type v} [EquivBEq α] [LawfulHashable α] (m : Raw₀ α (fun _ => β))
+omit [LawfulBEq α]
+
+-- @[simp]
+-- theorem modify_empty [EquivBEq α] [LawfulHashable α] {k : α} {f : β → β} :
+--     Const.modify empty k f = empty := by
+--   simp_to_model using List.Const.modify_empty
+
+-- theorem modify_of_not_mem [EquivBEq α] [LawfulHashable α] {k : α} {f g : β → β} (h : m.contains k = false) :
+--     Const.modify m k f = m := by
+--   simp_to_model using List.Const.modify_of_not_mem
 
 @[simp]
 theorem isEmpty_modify (m : Raw₀ α (fun _ => β)) (h : m.1.WF) {k : α} {f : β → β} :
     (Const.modify m k f).1.isEmpty = m.1.isEmpty := by
   simp_to_model using List.Const.isEmpty_modifyKey
 
+theorem contains_modify (h : m.1.WF) {k k' : α} {f : β → β} :
+    (Const.modify m k f).contains k' = m.contains k' := by
+  simp_to_model using List.Const.containsKey_modifyKey
+
+theorem size_modify (h : m.1.WF) {k : α} {f : β → β} :
+    (Const.modify m k f).1.size = m.1.size := by
+  simp_to_model using List.Const.length_modifyKey
+
+theorem get?_modify (h : m.1.WF) {k k' : α} {f : β → β} :
+    Const.get? (Const.modify m k f) k' = if k == k' then
+      (Const.get? m k).map f
+    else
+      Const.get? m k' := by
+  simp_to_model using List.Const.getValue?_modifyKey
+
 @[simp]
-theorem isEmpty_alter (m : Raw₀ α (fun _ => β)) (h : m.1.WF)  {k : α} {f : Option β → Option β} :
-    (Const.alter m k f).1.isEmpty ↔ (m.erase k).1.isEmpty ∧ f (Const.get? m k) = none := by
-  simp_to_model using List.Const.isEmpty_alterKey
+theorem get?_modify_self (h : m.1.WF) {k : α} {f : β → β} :
+    Const.get? (Const.modify m k f) k = (Const.get? m k).map f := by
+  simp_to_model using List.Const.getValue?_modifyKey_self
+
+theorem get_modify (h : m.1.WF) {k k' : α} {f : β → β}
+    (hc : (Const.modify m k f).contains k') :
+    Const.get (Const.modify m k f) k' hc =
+    if heq : k == k' then
+      haveI h' : m.contains k := by rwa [contains_modify _ h, ← contains_congr _ h heq] at hc
+      f (Const.get m k h')
+    else
+      haveI h' : m.contains k' := by rwa [contains_modify _ h] at hc
+      Const.get m k' h' := by
+  simp_to_model using List.Const.getValue_modifyKey
+
+@[simp]
+theorem get_modify_self (h : m.1.WF) {k : α} {f : β → β} {hc : (Const.modify m k f).contains k} :
+    haveI h' : m.contains k := by rwa [contains_modify _ h] at hc
+    Const.get (Const.modify m k f) k hc = f (Const.get m k h') := by
+  simp_to_model using List.Const.getValue_modifyKey_self
+
+theorem get!_modify (h : m.1.WF) {k k' : α} [hi : Inhabited β] {f : β → β} :
+    Const.get! (Const.modify m k f) k' =
+    if k == k' then
+      Const.get? m k |>.map f |>.get!
+    else
+      Const.get! m k' := by
+  simp_to_model using List.Const.getValue!_modifyKey
+
+@[simp]
+theorem get!_modify_self (h : m.1.WF) {k : α} [Inhabited (β)] {f : β → β} :
+    Const.get! (Const.modify m k f) k = ((Const.get? m k).map f).get! := by
+  simp_to_model using List.Const.getValue!_modifyKey_self
+
+theorem getD_modify (h : m.1.WF) {k k' : α} {v : β} {f : β → β} :
+    Const.getD (Const.modify m k f) k' v =
+    if k == k' then
+      Const.get? m k |>.map f |>.getD v
+    else
+      Const.getD m k' v := by
+  simp_to_model using List.Const.getValueD_modifyKey
+
+@[simp]
+theorem getD_modify_self (h : m.1.WF) {k : α} {v : β} {f : β → β} :
+    Const.getD (Const.modify m k f) k v = ((Const.get? m k).map f).getD v := by
+  simp_to_model using List.Const.getValueD_modifyKey_self
+
+theorem getKey?_modify (h : m.1.WF) {k k' : α} {f : β → β} :
+    (Const.modify m k f).getKey? k' =
+    if k == k' then
+      if m.contains k then some k else none
+    else
+      m.getKey? k' := by
+  simp_to_model using List.Const.getKey?_modifyKey
+
+theorem getKey?_modify_self (h : m.1.WF) {k : α} {f : β → β} :
+    (Const.modify m k f).getKey? k = if m.contains k then some k else none := by
+  simp_to_model using List.Const.getKey?_modifyKey_self
+
+theorem getKey!_modify (h : m.1.WF) [Inhabited α] {k k' : α} {f : β → β} :
+    (Const.modify m k f).getKey! k' =
+    if k == k' then
+      if m.contains k then k else panic ""
+    else
+      m.getKey! k' := by
+  simp_to_model using List.Const.getKey!_modifyKey
+
+theorem getKey!_modify_self (h : m.1.WF) [Inhabited α] {k : α} {f : β → β} :
+    (Const.modify m k f).getKey! k = if m.contains k then k else panic "" := by
+  simp_to_model using List.Const.getKey!_modifyKey_self
+
+theorem getKey_modify (h : m.1.WF) [Inhabited α] {k k' : α} {f : β → β}
+    (hc : (Const.modify m k f).contains k') :
+    (Const.modify m k f).getKey k' hc =
+    if heq : k == k' then
+      k
+    else
+      haveI h' : m.contains k' := by rwa [contains_modify _ h] at hc
+      m.getKey k' h' := by
+  simp_to_model using List.Const.getKey_modifyKey
+
+@[simp]
+theorem getKey_modify_self (h : m.1.WF) [Inhabited α] {k : α} {f : β → β}
+    (hc : (Const.modify m k f).contains k) : (Const.modify m k f).getKey k hc = k := by
+  simp_to_model using List.Const.getKey_modifyKey_self
+
+theorem getKeyD_modify (h : m.1.WF) {k k' d : α} {f : β → β} :
+    (Const.modify m k f).getKeyD k' d =
+    if k == k' then
+      if m.contains k then k else d
+    else
+      m.getKeyD k' d := by
+  simp_to_model using List.Const.getKeyD_modifyKey
+
+theorem getKeyD_modify_self (h : m.1.WF) [Inhabited α] {k d : α} {f : β → β} :
+    (Const.modify m k f).getKeyD k d = if m.contains k then k else d := by
+  simp_to_model using List.Const.getKeyD_modifyKey_self
 
 end Const
+
+end Modify
